src/num/theories/SingleStep.{sig,sml} is gone. The defininitions of Cases, Cases_on, Induct, Induct_on, CASE_TAC (and co.) are now in basicProof/BasicProvers. completeInduct_on and measureInduct_on are now in numLib. recInduct is now in src/tfl/Induction.sml. All these are collected in bossLib, so the changes should be invisible to ordinary users.
SingleStep.*.doc has been changed accordingly.

BasicProvers.NORM_TAC should now automatically perform
all case splits (from if-then-else expressions as
well as case expression) arising anywhere in the goal.

examples/dev/sw2/compiler.sig
@@ -3,6 +3,8 @@ sig
   include Abbrev
   (* val style : arm_code_format ref *)
   val f_compile : thm list -> ((thm * thm) list, thm list * thm list) Lib.verdict
-  val b_compile :  ((thm * thm) list, 'c) Lib.verdict -> ((thm * thm) list, 'c) Lib.verdict
+(*  val b_compile :  ((thm * thm) list, 'c) Lib.verdict -> ((thm * thm) list, 'c) Lib.verdict
   val pp_compile : thm list -> ((thm * thm) list, thm list * thm list) Lib.verdict
+*)
+
 end
